WIP: wtraced new causal

nondeterministic_dataflow/Wtraced_Composition.thy
@@ -4,33 +4,68 @@ imports
   "BNA_Operators"
 begin
 
+inductive visible_cause for wire where
+  "visible_cause wire buf (LCons (VInp (Inl p) x) ios) (LCons (VInp p x) ios1) ios2 buf ios ios1 ios2"
+| "visible_cause wire buf (LCons (VOut (Inr p) x) ios) ios1 (LCons (VOut p x) ios2) buf ios ios1 ios2"
+| "wire p = None \<Longrightarrow> visible_cause wire buf (LCons (VOut (Inl p) x) ios) (LCons (VOut p x) ios1) ios2 buf ios ios1 ios2"
+| "p \<notin> ran wire \<Longrightarrow> visible_cause wire buf (LCons (VInp (Inr p) x) ios) ios1 (LCons (VInp p x) ios2) buf ios ios1 ios2"
+| "visible_cause wire buf ios ios1 ios2 buf' ios ios1' ios2' \<Longrightarrow>
+   wire p = Some q \<Longrightarrow> visible_cause wire buf ios (LCons (VOut p x) ios1) ios2 (BENQ q x buf') ios ios1' ios2'"
+| "visible_cause wire buf ios ios1 ios2 buf' ios ios1' ios2' \<Longrightarrow>
+   p \<in> ran wire \<Longrightarrow> buf' p \<noteq> [] \<Longrightarrow> BHD p buf' = x \<Longrightarrow>
+   visible_cause wire buf ios ios1 (LCons (VInp p x) ios2) (BTL p buf') ios' ios1' ios2'"
 
 coinductive causal for wire where
-  "causal wire buf LNil LNil"
-| "causal wire buf ios1 ios2 \<Longrightarrow> causal wire buf (LCons (VInp p x) ios1) ios2"
-| "causal wire buf ios1 ios2 \<Longrightarrow> wire p = None \<Longrightarrow> causal wire buf (LCons (VOut p x) ios1) ios2"
+ "causal wire buf' ios' ios1' ios2' \<Longrightarrow> visible_cause wire buf ios ios1 ios2 buf' ios' ios1' ios2' \<Longrightarrow> causal wire buf ios ios1 ios2"
+(* | "causal wire buf ios1 ios2 \<Longrightarrow> wire p = None \<Longrightarrow> causal wire buf (LCons (VOut p x) ios1) ios2"
 | "causal wire (BENQ q x buf) ios1 ios2 \<Longrightarrow> wire p = Some q \<Longrightarrow> causal wire buf (LCons (VOut p x) ios1) ios2"
 | "causal wire buf ios1 ios2 \<Longrightarrow> causal wire buf ios1 (LCons (VOut p y) ios2)"
 | "causal wire buf ios1 ios2 \<Longrightarrow> p \<notin> ran wire \<Longrightarrow> causal wire buf ios1 (LCons (VInp p y) ios2)"
-| "causal wire (BTL p buf) ios1 ios2 \<Longrightarrow> buf p \<noteq> [] \<Longrightarrow> y = BHD p buf \<Longrightarrow> p \<in> ran wire \<Longrightarrow> causal wire buf ios1 (LCons (VInp p y) ios2)"
+| "causal wire (BTL p buf) ios1 ios2 \<Longrightarrow> buf p \<noteq> [] \<Longrightarrow> y = BHD p buf \<Longrightarrow> p \<in> ran wire \<Longrightarrow> causal wire buf ios1 (LCons (VInp p y) ios2)" *)
+(* 
 
 abbreviation "VIO_Inls ios \<equiv>
-  lmap (case_VIO (case_sum VInp undefined) (case_sum VOut undefined)) (lfilter (case_VIO (case_sum \<top> \<bottom>) (case_sum \<top> \<bottom>)) ios)"
+  lmap (case_VIO (case_sum VInp VInp) (case_sum VOut VOut)) (lfilter (case_VIO (case_sum \<top> \<bottom>) (case_sum \<top> \<bottom>)) ios)"
 
 abbreviation "VIO_Inrs ios \<equiv>
-  lmap (case_VIO (case_sum undefined VInp) (case_sum undefined VOut)) (lfilter (case_VIO (case_sum \<bottom> \<top>) (case_sum \<bottom> \<top>)) ios)"
+  lmap (case_VIO (case_sum VInp VInp) (case_sum VOut VOut)) (lfilter (case_VIO (case_sum \<bottom> \<top>) (case_sum \<bottom> \<top>)) ios)"
 
 abbreviation visible_VIO where "visible_VIO wire io \<equiv> case_VIO (\<lambda>p _. case_sum (\<lambda> _. True) (\<lambda> q. q \<notin> ran wire) p) (\<lambda> p _. case_sum (\<lambda> q. q \<notin> dom wire) (\<lambda> _. True) p) io" 
 
-inductive_cases causal_VInpInlE[elim]: "causal wire buf (LCons (VInp p x) ios1') ios2"
+lemma causal_LCons_VInp_Inl:
+  "causal wire buf (LCons (VInp p x) ios1) ios2 \<Longrightarrow>
+   causal wire buf ios1 ios2"
+  apply (coinduction arbitrary: buf ios1 ios2 rule: causal.coinduct)
+  subgoal for buf ios1 ios2
+    apply (erule causal.cases)
+          apply simp_all
+    apply hypsubst_thin
+    apply (smt (verit) causal.cases)
+    done
+  done
+
+lemma causal_LCons_VOut_Inr:
+  "causal wire buf ios (LCons (VOut p x) ios2) \<Longrightarrow>
+   causal wire buf ios1 ios2"
+  apply (coinduction arbitrary: buf ios1 ios2 rule: causal.coinduct)
+  subgoal for buf ios1 ios2
+    apply (erule causal.cases)
+          apply simp_all
+    apply hypsubst_thin
+    oops *)
+
+lemma visible_cause_VInp_Inl_LNil_False:
+  "visible_cause wire buf (LCons (VInp (Inl lp) x) ios) ios1 ios2 buf' ios' ios1' ios2' \<Longrightarrow>
+   ios1 = LNil \<Longrightarrow>
+   False"
+  apply (induct buf "LCons (VInp (Inl lp) x) ios" ios1 ios2 buf' ios' ios1' ios2' pred: visible_cause)
+    apply auto
+  done
 
 
 lemma
   "wtraced (comp_op wire buf op1 op2) ios = 
-   (\<exists> ios1 ios2. wtraced op1 ios1 \<and> wtraced op2 ios2 \<and>
-    lfilter (case_VIO \<top> (\<lambda> p _. p \<notin> ran wire)) ios1 = VIO_Inls ios \<and>
-    lfilter (case_VIO (\<lambda> p _. p \<notin> dom wire) \<top>) ios2 = VIO_Inrs ios \<and>
-    causal wire buf ios1 ios2)"
+   (\<exists> ios1 ios2. wtraced op1 ios1 \<and> wtraced op2 ios2 \<and> causal wire buf ios ios1 ios2)"
   apply (rule iffI)
   subgoal
     sorry
@@ -53,21 +88,64 @@ lemma
               apply hypsubst_thin
               apply (erule wtraced.cases)
               subgoal
+              apply (erule causal.cases)
+                apply auto
+                apply hypsubst_thin
+                using visible_cause_VInp_Inl_LNil_False apply fast
+                done
+              subgoal
+                apply hypsubst_thin
+         apply (erule causal.cases)
+                apply auto
+                sorry
+              done
+            subgoal for rp
+         apply (simp split: if_splits)
+              apply hypsubst_thin
+              apply rotate_tac
+              apply (erule wtraced.cases)
+              subgoal sorry
+              subgoal
+                apply hypsubst_thin
+    apply (erule causal.cases)
+                apply auto
+
+end
                 by simp
               subgoal for vio op op' ios1'
                 apply (simp split: if_splits)
-                 apply hypsubst_thin
                 subgoal
-                  apply (erule causal_VInpInlE)
-                        apply auto
-                     apply hypsubst_thin
-                  subgoal
+                 apply hypsubst_thin
+                  apply (drule causal_LCons_VInp_Inl)
                     apply (intro exI conjI)
                      apply (rule wstep_comp_op_L_Inp)
                        apply assumption
                       apply (rule refl)+
                     apply blast
-                    done
+                  done
+                subgoal
+                 apply hypsubst_thin
+                  apply (simp split: VIO.splits)
+                  subgoal for p x
+                  apply (intro exI conjI)
+                     apply (rule wstep_trans(2)[of _ "comp_op wire (BENQ p x buf) op' op2"])
+                    unfolding wstep_def
+                    subgoal sorry
+              
+
+                    find_theorems wtraced wstep
+
+
+end
+                  apply (rule step_Tau_comp_op_L)
+
+                  find_theorems wstep name: trans
+
+
+
+end
+
+
                   subgoal for ios2 p y
                     apply hypsubst_thin
                     apply (intro exI conjI)
@@ -79,7 +157,15 @@ lemma
                       apply (rule refl)+
                         apply assumption+
                      apply fastforce
-                        apply (rule causal.intros(5))
+                    apply (rule causal.intros(5)) 
+                    apply (rule causal_LCons_VInp_Inl)
+                    apply force
+                    done
+                  subgoal for ios2 p y
+                    apply hypsubst_thin
+                    sledgehammer             
+
+                    find_theorems "ldropWhile _ _ = LCons _ _"
 
         find_theorems lfilter LNil
 
